scan_lib.v
@@ -1005,4 +1005,132 @@ Ltac prove_precise :=
       end; sep_split_in Hsat; sep_split_in Hsat')
   end.
 Hint Resolve is_array_precise precise_emp.
+Require Import LibTactics Psatz.
+Lemma conj_xs_init_flatten l1 l2 f_ini :
+  forall s stk,
+    stk ||=
+      conj_xs (ls_init s l1 (fun i =>
+        conj_xs (ls_init 0 l2 (fun j => f_ini (j + i * l2))))) <=>
+      conj_xs (ls_init (s * l2) (l1 * l2) (fun i => f_ini i)).
+Proof.
+  induction l1; simpl; [reflexivity|].
+  introv.
+  Lemma ls_init_app {T : Type} l1 l2 (f_ini : nat -> T) :
+    forall s, 
+      ls_init s (l1 + l2) f_ini = ls_init s l1 f_ini ++ ls_init (s + l1) l2 f_ini.
+  Proof.
+    induction l1; simpl.
+    - introv; rewrite <-plus_n_O; reflexivity.
+    - introv; f_equal.
+      rewrite IHl1; do 2 f_equal; ring.
+  Qed.
+  rewrite ls_init_app, conj_xs_app.
+  apply star_proper.
+  eapply equiv_from_nth; rewrite !init_length; eauto.
+  - intros i Hi stk'; repeat rewrite (@ls_init_spec _ _ _ emp); destruct lt_dec.
+    cutrewrite (0 + i + s * l2 = s * l2 + i); [|ring]; reflexivity.
+    reflexivity.
+  - rewrite IHl1.
+    cutrewrite (S s * l2 = s * l2 + l2); [|ring]; reflexivity.
+Qed.
+Lemma conj_xs_init_flatten0 l1 l2 f_ini :
+  forall stk,
+    stk ||=
+      conj_xs (ls_init 0 l1 (fun i =>
+        conj_xs (ls_init 0 l2 (fun j => f_ini (j + i * l2))))) <=>
+      conj_xs (ls_init 0 (l1 * l2) (fun i => f_ini i)).      
+Proof.
+  cutrewrite (0 = 0 * l2); [|omega].
+  introv; rewrite <-conj_xs_init_flatten.
+  reflexivity.
+Qed.
+Lemma is_array_skip_arr E n m len' f_ini :
+  n <> 0 -> m <> 0 ->
+  forall stk, stk ||= 
+    is_array E len' f_ini 0 <=>
+    conj_xs (ls_init 0 n (fun i =>
+      conj_xs (ls_init 0 m (fun j =>
+        skip_arr E 0 len' (n * m) f_ini (j + i * m))))).
+Proof.
+  intros.
+  rewrite conj_xs_init_flatten0.
+  lets Heq: (>>distribute_correct (n * m) (nt_step (n * m))); rewrite Heq; clear Heq.
+  2: unfold nt_step; intros; apply Nat.mod_upper_bound; nia.
+  eapply (@equiv_from_nth emp).
+  rewrite init_length, distribute_length; ring.
+  rewrite distribute_length; intros i Hi stk'.
+  rewrite ls_init_spec; destruct lt_dec; try omega.
+  reflexivity.
+Qed.
 
+Lemma CSLp_backward (P' P : assn) n E C Q : 
+  CSLp n E P C Q -> (P' |= P) -> CSLp n E P' C Q.
+Proof.
+  unfold CSLp; intros Hcsl Hp; intros.
+  exploit Hcsl.
+  eauto.
+  eauto.
+  unfold sat_k in *.
+  instantiate (1:=h).
+  instantiate (1:=leqks).
+  destruct low_eq_repr.
+  apply Hp; eauto.
+  intros; eauto.
+Qed.  
+
+Lemma safe_gl_forward n m E ks h (Q Q' : assn) : 
+  @safe_nk n E m ks h Q -> 
+  (Q |= Q') ->
+  @safe_nk n E m ks h Q'.
+Proof.
+  revert h ks; induction m; simpl; intros h ks Hsafe Hq; eauto.
+  simpl in Hsafe; destructs Hsafe.
+  repeat split; eauto.
+  - intros; unfold sat_k in *.
+    exploit H; eauto.
+    intros [x ?]; exists x.
+    destruct low_eq_repr; apply Hq; eauto.
+  - exploit H2; eauto.
+    intros; jauto.
+  - exploit H2; eauto.
+    intros; jauto.
+  - intros; exploit H3; eauto.
+    intros (h'' & ? & ? & ?); exists h''; repeat split; eauto.
+Qed.  
+
+Lemma CSLp_forward P n E C (Q Q' : assn) : 
+  CSLp n E P C Q -> (Q |= Q') -> CSLp n E P C Q'.
+Proof.
+  unfold CSLp; intros; applys safe_gl_forward; eauto.
+Qed.
+
+Lemma inde_conj_xs assns vs :
+  (forall i, i < length assns -> inde (nth i assns emp) vs) ->
+  inde (conj_xs assns) vs.
+Proof.
+  induction assns; simpl; try omega.
+  - intros; unfold_conn; unfold inde; eauto; simpl; tauto.
+  - intros H.
+    apply inde_sconj; eauto.
+    + specialize (H 0); simpl in H; apply H; omega.
+    + apply IHassns; intros i Hi; specialize (H (S i)); simpl in H; apply H; omega.
+Qed.
+
+Lemma low_assn_conj_xs assns E :
+  (forall i, i < length assns -> low_assn E (nth i assns emp)) ->
+  low_assn E (conj_xs assns) .
+Proof.
+  induction assns; simpl; intros; repeat prove_low_assn.
+  specialize (H 0); apply H; omega.
+  apply IHassns; intros i; specialize (H (S i)); intros; apply H; omega.
+Qed.
+
+Lemma has_no_vars_conj_xs assns :
+  (forall i, i < length assns -> has_no_vars (nth i assns emp)) ->
+  has_no_vars (conj_xs assns).
+Proof.
+  induction assns; simpl; intros; repeat has_no_vars_assn.
+  apply (H 0); omega.
+  apply IHassns; intros i; specialize (H (S i)); simpl in *.
+  intros; apply H; omega.
+Qed.
